Problem 18: Compute $\displaystyle\sum_{n=1}^\infty \frac{6^n}{(3^{n+1}-2^{n+1})(3^n-2^n)}$.

Solution:

\begin{align*}
\sum_{n = 1}^{\infty} \frac{6^n}{(3^{n+1} - 2^{n+1})(3^n - 2^n)} &= \lim_{k \rightarrow \infty} \sum_{n = 1}^{k} \frac{6^n}{(3^{n+1} - 2^{n+1})(3^n - 2^n)} \\
&= \lim_{k \rightarrow \infty} \sum_{n = 1}^{k} \left( \frac{A}{3^{n+1} - 2^{n+1}} + \frac{B}{3^n - 2^n} \right) \\
\end{align*}

Now let's find solutions for A and B.

\begin{align*}
\frac{A}{3^{n+1} - 2^{n+1}} + \frac{B}{3^n - 2^n} &= \frac{6^n}{(3^{n+1} - 2^{n+1})(3^n - 2^n)} \\ \\
\frac{A(3^n - 2^n)}{(3^{n+1} - 2^{n+1})(3^n - 2^n)} + \frac{B(3^{n+1} - 2^{n+1}) }{(3^{n+1} - 2^{n+1})(3^n - 2^n)} &= \frac{6^n}{(3^{n+1} - 2^{n+1})(3^n - 2^n)} \\ \\
A(3^n - 2^n) + B(3^{n+1} - 2^{n+1}) = 6^n \\ \\
A3^n - A2^n + B3^{n+1} - B2^{n+1} = 6^n \\ \\
3^n(A + 3B) - 2^n(A + 2B) = 6^n \\ \\
\end{align*}

We can set $A + 3B = 2^n$ and $A + 2B = 0$.

\begin{align*}
A + 3B &= 2^n \\
A + 2B &= 0 \\
B &= 2^n \\
A &= -2^{n+1}
\end{align*}

Now let's plug in A and B.

\begin{align*}
\sum_{n = 1}^{\infty} \frac{6^n}{(3^{n+1} - 2^{n+1})(3^n - 2^n)}
&= \lim_{k \rightarrow \infty} \sum_{n = 1}^{k} \left( \frac{A}{3^{n+1} - 2^{n+1}} + \frac{B}{3^n - 2^n} \right) \\
&= \lim_{k \rightarrow \infty} \sum_{n = 1}^{k} \left( \frac{-2^{n+1}}{3^{n+1} - 2^{n+1}} + \frac{2^n}{3^n - 2^n} \right) \\
&= \lim_{k \rightarrow \infty} \sum_{n = 1}^{k} \left( \frac{2^n}{3^n - 2^n} - \frac{2^{n+1}}{3^{n+1} - 2^{n+1}} \right) \\
&= \lim_{k \rightarrow \infty} \left( \frac{2}{3 - 2} - \frac{2^{k+1}}{3^{k+1} - 2^{k+1}} \right) \\
&= \lim_{k \rightarrow \infty} \frac{2}{3-2} - \lim_{k \rightarrow \infty} \frac{2^{k+1}}{3^{k+1} - 2^{k+1}} \\
&= 2 - \lim_{k \rightarrow \infty} \frac{2^{k+1}}{3^{k+1} - 2^{k+1}} \\
&= 2 - \lim_{k \rightarrow \infty} \frac{1}{(\frac{3}{2})^{k+1} - 1} \\
&= 2 - 0 \\
&= \boxed{2}
\end{align*}
