Problem 13: Find the slope of the tangent line to $r = 3 \cos 2\theta$ at $\theta = \dfrac{\pi}{3}$.

(Source: AoPS Calculus)

We will use the formula $\dfrac{dy}{dx} = \dfrac{dy/d\theta}{dx/d\theta}$.

From our knowledge of polar coordinates, we know that $y = r \sin \theta$ and $x = r \cos \theta$. Since $r$ is a function of $\theta$ (and not a constant) we will have to use the product rule when differentiating these equations.

\begin{align*}
\dfrac{dy}{dx} &= \dfrac{dy/d\theta}{dx/d\theta} \\
&= \dfrac{r' \sin \theta + r \cos \theta}{r' \cos \theta - r \sin \theta} \\
&= \dfrac{r' \sin \theta + r \cos \theta}{r' \cos \theta - r \sin \theta} \\
\end{align*}

Now we have $r' = -6 \sin 2 \theta$ by the chain rule. Substituting for $r$ and $r'$, we get

\begin{align*}
\dfrac{dy}{dx} &= \dfrac{r' \sin \theta + r \cos \theta}{r' \cos \theta - r \sin \theta} \\
&= \dfrac{\left(-6 \sin 2 \theta\right)\left(\sin \theta\right) + \left(3 \cos 2\theta\right)\left(\cos \theta\right)}{\left(-6 \sin 2 \theta\right)\left(\cos \theta\right) - \left(3 \cos 2\theta\right)\left(\sin \theta\right)} \\
\end{align*}

We arrive at an equation for the slope of the tanget line in terms of the variable $\theta$. We can plug in $\theta = \dfrac{\pi}{3}$ to get the slope of the tangent line at $\dfrac{\pi}{3}$ radians.

\begin{align*}
\dfrac{dy}{dx} \left(\dfrac{\pi}{3}\right) &= \dfrac{\left(-6 \sin \dfrac{2\pi}{3}\right)\left(\sin \dfrac{\pi}{3} \right) + \left(3 \cos \dfrac{2\pi}{3}\right)\left(\cos \dfrac{\pi}{3} \right)}{\left(-6 \sin \dfrac{2\pi}{3}\right)\left(\cos \dfrac{\pi}{3}\right) - \left(3 \cos \dfrac{2\pi}{3}\right)\left(\sin \dfrac{\pi}{3}\right)} \\
&= \dfrac{\left( -3 \sqrt3 \right)\left(\dfrac{\sqrt3}{2} \right) + \left( -\dfrac{3}{2}\right)\left(\dfrac{1}{2} \right)}{\left(-3 \sqrt3\right)\left(\dfrac{1}{2}\right) - \left(-\dfrac{3}{2}\right)\left(\dfrac{\sqrt3}{2}\right)} \\
&= \dfrac{\left(-\dfrac{18}{4} \right) + \left( -\dfrac{3}{4}\right)}{\left(-\dfrac{6\sqrt3}{4}\right) + \left(\dfrac{3 \sqrt 3}{4}\right)} \\
&= \dfrac{-18 + -3}{-6\sqrt3 + 3 \sqrt 3} \\
&= \dfrac{-21}{-3\sqrt3} \\
&= \dfrac{7}{\sqrt3} \\
&= \boxed{\dfrac{7 \sqrt 3}{3}} \\
\end{align*}

The slope of the tangent line at $\theta = \dfrac{\pi}{3}$ is $\boxed{\dfrac{7 \sqrt 3}{3}}$.
